theories/Dynamics/Term.v
@@ -1,4 +1,4 @@
-From Metaconfigurations Require Import Syntax.Term Syntax.Ty Syntax.Value Object Process.
+From Metaconfigurations Require Import Map Syntax.Term Syntax.Ty Syntax.Value Object Process.
 From stdpp Require Import base.
 
 Reserved Notation "⟨ ϵ, σ, e ⟩ ⇓ v" (at level 80, no associativity).
@@ -15,5 +15,6 @@ Section Eval.
 
   Variable π : Π.
 
-  Inductive eval : Term.t Π Ω π → Value.t → Prop :=
+  Inductive eval : (∀ ω, ) Term.t Π Ω π → Value.t → Prop :=
     | 
+End Eval.
